@prefix cc: <http://creativecommons.org/ns#> .
@prefix dash: <http://datashapes.org/dash#> .
@prefix dcterms: <http://purl.org/dc/terms/> .
@prefix owl: <http://www.w3.org/2002/07/owl#> .
@prefix rdf: <http://www.w3.org/1999/02/22-rdf-syntax-ns#> .
@prefix rdfs: <http://www.w3.org/2000/01/rdf-schema#> .
@prefix sh: <http://www.w3.org/ns/shacl#> .
@prefix skos: <http://www.w3.org/2004/02/skos/core#> .
@prefix swa: <http://topbraid.org/swa#> .
@prefix tosh: <http://topbraid.org/tosh#> .
@prefix xml: <http://www.w3.org/XML/1998/namespace> .
@prefix xsd: <http://www.w3.org/2001/XMLSchema#> .
@prefix rde: <https://github.com/buda-base/rdf-document-editor/> .

rde:allowPushToTopLevelLabel
  a owl:ObjectProperty ;
  rdfs:label "allow UI to push objects of this property to top level label"@en ;
  rdfs:domain sh:PropertyShape ;
  skos:definition "Indicates that the editor should allow the user to copy the object of this property as the label of the top level entity. Implementation is not specified further."@en ;
.

rde:uniqueValueAmongSiblings
  a owl:DatatypeProperty ;
  rdfs:label "unique among siblings"@en ;
  rdfs:domain sh:PropertyShape ;
  rdfs:range xsd:boolean ;
  skos:definition "true indicates that siblings should each have a different value for the object of this property."@en ;
.

rde:readOnly
  a owl:DatatypeProperty ;
  rdfs:label "read only"@en ;
  rdfs:domain sh:PropertyShape ;
  rdfs:range xsd:boolean ;
  skos:definition "true indicates that the editor should not allow the user to change the property"@en ;
.

rde:defaultValue
  a owl:DatatypeProperty ;
  rdfs:label "editor default value"@en ;
  rdfs:domain sh:PropertyShape ;
  skos:definition "indicates the default value that the editor should display when there is no value"@en ;
.

rde:defaultLanguage
  a owl:DatatypeProperty ;
  rdfs:label "default language"@en ;
  rdfs:domain sh:PropertyShape ;
  rdfs:range xsd:string ;
  skos:definition "indicates the default language that the editor should display for the values of a certain property"@en ;
.

rde:connectIDs
  a owl:DatatypeProperty ;
  rdfs:label "connect IDs"@en ;
  rdfs:domain sh:PropertyShape ;
  rdfs:range xsd:boolean ;
  skos:definition "When creating a new object of this (external) property, the URI should be connected to the one of the current subject. The nature of the connection is left to the implementation. One example is if a user creates edits the instance ex:MW123 and creates a new work, the new work would be ex:WA123."@en ;
.

rde:copyObjectsOfProperty
  a owl:ObjectProperty ;
  rdfs:label "copy objects of property"@en ;
  rdfs:domain sh:PropertyShape ;
  rdfs:range rdf:Property ;
  skos:definition "when creating a new object of this (external) property, automatically copy triples with the object of this property (typically skos:prefLabel) as predicates"@en ;
.

rde:allowBatchManagement
  a owl:DatatypeProperty ;
  rdfs:label "allow batch management"@en ;
  rdfs:domain sh:PropertyShape ;
  rdfs:range xsd:boolean ;
  skos:definition "instructs the UI to allow batch creation / removal of objects of this property. The implementation is not normalized. In RDE this makes the editor add a button to create multiple volume objects when the user edits an instance."@en ;
.

rde:identifierPrefix
  a owl:DatatypeProperty ;
  rdfs:label "prefix for resource id"@en ;
  rdfs:range xsd:string ;
  skos:definition "local name prefix to use when generating a new URI for a resource."@en ;
.

rde:displayPriority
  a owl:DatatypeProperty ;
  rdfs:label "display priority"@en ;
  rdfs:range xsd:integer ;
  rdfs:domain sh:PropertyShape ;
  skos:definition "indicates if a property should be displayed or hidden, using a number between 0 and 2 where 0 means the property should always be displayed, 1 means the property can be hidden behind a see more button if necessary, 2 means the property should be hidden unless there's an associated value, and 3 means that the property should always be hidden (use for inferred fields for instance)."@en ;
.

rde:classIn
  a owl:DatatypeProperty ;
  rdfs:label "expected object type"@en ;
  rdfs:domain rdfs:Resource ;
  skos:definition "this is similar to sh:class except that the constraint is that the type must be any of the listed types instead of the conjuction of all listed types. The object should be a rdf:list."@en ;
.

rde:independentIdentifiers
  a owl:DatatypeProperty ;
  rdfs:label "independent identifiers"@en ;
  rdfs:domain sh:NodeShape ;
  rdfs:range xsd:boolean ;
  skos:definition "the identifiers for the resource are independent from its parent resource."@en ;
.

rde:sortOnProperty
  a owl:ObjectProperty ;
  rdfs:label "sort on property"@en ;
  rdfs:domain sh:PropertyShape ;
  skos:definition "sort the objects of the property shape by one of their property. This is for display purpose only and has no effect on the data."@en ;
.

rde:allowMarkDown
  a owl:DatatypeProperty ;
  rdfs:label "node shape type"@en ;
  rdfs:domain sh:PropertyShape ;
  rdfs:range xsd:boolean ;
  skos:definition "the editor displays a markdown editor for the objects of this property"@en ;
.

rde:ShapeType
  a owl:Class ;
.

rde:nodeShapeType
  a owl:ObjectProperty ;
  rdfs:label "node shape type"@en ;
  rdfs:domain sh:NodeShape ;
  rdfs:range rde:ShapeType ;
.

rde:propertyShapeType
  a owl:ObjectProperty ;
  rdfs:label "node shape type"@en ;
  rdfs:domain sh:PropertyShape ;
  rdfs:range rde:ShapeType ;
.

rde:increment
  a owl:DatatypeProperty ;
  rdfs:label "increment by"@en ;
  rdfs:domain sh:PropertyShape ;
  rdfs:range xsd:integer ;
  skos:definition "an amount to increment the value of the sh:path property by"@en ;
.

rde:ExternalShape
  a rde:ShapeType ;
  rdfs:label "external shape"@en ;
  skos:definition "the shape refers to resource external to the document"@en ;
.

rde:InternalShape
  a rde:ShapeType ;
  rdfs:label "internal shape"@en ;
  skos:definition "the shape refers to a resource within the document"@en ;
.

# defining the path to use in the list path pattern (https://www.topquadrant.com/constraints-on-rdflists-using-shacl/)

rde:listPathZeroOrMore sh:zeroOrMorePath rdf:rest .
rde:listPath rdf:first rde:listPathZeroOrMore ;
             rdf:rest rdf:first
.

rde:specialPattern
  a owl:ObjectProperty ;
  rdfs:domain sh:PropertyShape ;
  rdfs:range rde:SpecialPattern ;
  skos:prefLabel "special pattern"@en ;
  skos:definition "a complex pattern that a litteral argument should be checked against. Implementation is nor normalized."@en ;
.

rde:SpecialPattern
  a owl:Class ;
.

rde:PatternEDTF
  a rde:SpecialPattern ;
  skos:prefLabel "EDTF pattern"@en ;
  skos:description "Extended Date/Time Format (EDTF) has been designed by the Library of Congress and integrated into ISO8601-2019"@en ;
  rdfs:seeAlso <https://www.loc.gov/standards/datetime/> ;
.
rde:PatternISBN
  a rde:SpecialPattern ;
  skos:prefLabel "ISBN pattern"@en ;
