@prefix cc: <http://creativecommons.org/ns#> .
@prefix dash: <http://datashapes.org/dash#> .
@prefix dcterms: <http://purl.org/dc/terms/> .
@prefix owl: <http://www.w3.org/2002/07/owl#> .
@prefix rdf: <http://www.w3.org/1999/02/22-rdf-syntax-ns#> .
@prefix rdfs: <http://www.w3.org/2000/01/rdf-schema#> .
@prefix sh: <http://www.w3.org/ns/shacl#> .
@prefix skos: <http://www.w3.org/2004/02/skos/core#> .
@prefix swa: <http://topbraid.org/swa#> .
@prefix tosh: <http://topbraid.org/tosh#> .
@prefix xml: <http://www.w3.org/XML/1998/namespace> .
@prefix xsd: <http://www.w3.org/2001/XMLSchema#> .
@prefix rde: <https://github.com/buda-base/rdf-document-editor/> .

rde:allowPushToTopLevelLabel
  a owl:DatatypeProperty ;
  rdfs:label "allow push to top level skos pref label"@en ;
  rdfs:domain sh:PropertyShape ;
  rdfs:range xsd:boolean ;
  skos:definition "true indicates that the editor should allow the user to copy the object of this property as a label of the main entity of the document"@en ;
.

rde:readOnly
  a owl:DatatypeProperty ;
  rdfs:label "read only"@en ;
  rdfs:domain sh:PropertyShape ;
  rdfs:range xsd:boolean ;
  skos:definition "true indicates that the editor should not allow the user to change the property"@en ;
.
rde:defaultValue
  a owl:DatatypeProperty ;
  rdfs:label "editor default value"@en ;
  rdfs:domain sh:PropertyShape ;
  skos:definition "indicates the default value that the editor should display when there is no value"@en ;
.
rde:defaultLanguage
  a owl:DatatypeProperty ;
  rdfs:label "default language"@en ;
  rdfs:domain sh:PropertyShape ;
  rdfs:range xsd:string ;
  skos:definition "indicates the default language that the editor should display for the values of a certain property"@en ;
.

rde:connectIDs
  a owl:DatatypeProperty ;
  rdfs:label "connect IDs"@en ;
  rdfs:domain sh:PropertyShape ;
  rdfs:range xsd:boolean ;
  skos:definition "when creating a new object of this (external) property, the URI should be connected to the one of the current subject."@en ;
.
rde:copyObjectsOfProperty
  a owl:ObjectProperty ;
  rdfs:label "connect IDs"@en ;
  rdfs:domain sh:PropertyShape ;
  rdfs:range rdf:Property ;
  skos:definition "when creating a new object of this (external) property, automatically copy triples with the object of this property (typically skos:prefLabel) as predicates"@en ;
.
rde:allowBatchManagement
  a owl:DatatypeProperty ;
  rdfs:label "allow batch management"@en ;
  rdfs:domain sh:PropertyShape ;
  rdfs:range xsd:boolean ;
  skos:definition "instructs the UI to allow batch creation / removal of objects of this property"@en ;
.
rde:identifierPrefix
  a owl:DatatypeProperty ;
  rdfs:label "prefix for resource id"@en ;
  rdfs:range xsd:string ;
  skos:definition "prefix to use when generating identifier for a resource"@en ;
.
rde:displayPriority
  a owl:DatatypeProperty ;
  rdfs:label "display priority"@en ;
  rdfs:range xsd:integer ;
  rdfs:domain sh:PropertyShape ;
  skos:definition "indicates if a property should be displayed or hidden, using a number between 0 and 2 where 0 means the property should always be displayed, 1 means the property can be hidden behind a see more button if necessary, 2 means the property should be hidden unless there's an associated value, and 3 means that the property should always be hidden (use for inferred fields for instance)."@en ;
.
rde:classIn
  a owl:DatatypeProperty ;
  rdfs:label "expected object type"@en ;
  rdfs:domain rdfs:Resource ;
  skos:definition "this is similar to sh:class except that the constraint is that the type must be any of the listed types instead of the conjuction of all listed types. The object should be a rdf:list."@en ;
.
rde:nodeShapeType
  a owl:ObjectProperty ;
  rdfs:label "node shape type"@en ;
  rdfs:domain sh:NodeShape ;
  rdfs:range rde:ShapeType ;
  skos:definition "type of a node shape to discriminate among fact shapes, internal shapes, and so on"@en ;
.
rde:propertyShapeType
  a owl:ObjectProperty ;
  rdfs:label "node shape type"@en ;
  rdfs:domain sh:PropertyShape ;
  rdfs:range rde:ShapeType ;
  skos:definition "type of a node shape to discriminate among fact shapes, internal shapes, and so on"@en ;
.
rde:allowMarkDown
  a owl:DatatypeProperty ;
  rdfs:label "node shape type"@en ;
  rdfs:domain sh:PropertyShape ;
  rdfs:range xsd:boolean ;
  skos:definition "the object of the property can be in markdown"@en ;
.
rde:ShapeType
  a owl:Class ;
.
rde:independentIdentifiers
  a owl:DatatypeProperty ;
  rdfs:label "independent identifiers"@en ;
  rdfs:domain sh:NodeShape ;
  rdfs:range xsd:boolean ;
  skos:definition "the identifiers for the resource are independent from its parent resource"@en ;
.
rde:sortOnProperty
  a owl:ObjectProperty ;
  rdfs:label "sort on property"@en ;
  rdfs:domain sh:PropertyShape ;
  skos:definition "sort the objects of the property shape by one of their property. This is for display purpose only and has no effect on the data."@en ;
.
rde:ExternalShape
  a rde:ShapeType ;
  rdfs:label "node shape refers to resource external to focus node graph"@en ;
  skos:definition "this shape indicates external resource that is not contained in the focus node graph"@en ;
.
rde:FacetShape
  a rde:ShapeType ;
  rdfs:label "node shape is a facet"@en ;
  skos:definition "this shape applies to a resource contained in the graph of root Resource that is a facet of the containing resource"@en ;
.
rde:IgnoreShape
  a rde:ShapeType ;
  rdfs:label "node shape is ignored for editing"@en ;
  skos:definition "this shape indicates internal resource that is not editable"@en ;
.
